Use vectors for reactor-container's IO and state.

src/determinism.lean
@@ -1,65 +1,84 @@
 import basic
+import data.vector
 
-namespace determinism 
-  
-  def state := identifier → value  
-  def ports := identifier → value 
-  def env := state × ports
+namespace hidden 
+
+  variables i o s i' o' s' : ℕ 
+
+  -- CONTAINER
+
+  def inputs := vector value i
+  def outputs := vector value o
+  def state := vector value s
+  def container := (inputs i) × (outputs o) × (state s)
 
   -- REACTION
 
-  def reaction := env → env
+  def reaction := (container i o s) → (container i o s)
   
   namespace reaction
 
-    def determinism (r : reaction) : Prop := ∀ e₁ e₂ : env, e₁ = e₂ → r e₁ = r e₂
+    def determinism {i o s : ℕ} (r : reaction i o s) : Prop := 
+      ∀ c₁ c₂ : (container i o s), c₁ = c₂ → r c₁ = r c₂
 
-    theorem deterministic (r : reaction) : determinism r :=
-      assume (e₁ e₂ : env) (h : e₁ = e₂),
-      show r e₁ = r e₂, from congr_arg r h
+    theorem deterministic (r : reaction i o s) : determinism r :=
+      assume c₁ c₂ : container i o s,
+      assume h : c₁ = c₂,
+      show r c₁ = r c₂,
+      from congr_arg r h
 
   end reaction
 
-  -- NETWORK
+  -- BODY
 
-  -- The order produced by a network only describes the *priority* of the reactions, not their connections.
-  inductive network
-    | single (r : reaction) : network
-    | composed (head : reaction) (tail : network) : network
+  -- The order produced by a body only describes the *priority* of the reactions, not their connections.
+  inductive body
+    | single (r : reaction i o s) : body
+    | composed (head : reaction i o s) (tail : body) : body
 
-  namespace network
+  namespace body
 
-    def process : env → network → env
-      | e (network.single r) := r e
-      | e (network.composed h t) := process (h e) t
+    def process {i o s : ℕ} : (container i o s) → (body i o s) → (container i o s)
+      | c (body.single r) := r c
+      | c (body.composed h t) := process (h c) t
 
-    def determinism (n : network) : Prop := ∀ e₁ e₂ : env, e₁ = e₂ → process e₁ n = process e₂ n
+    def determinism {i o s : ℕ} (b : body i o s) : Prop := 
+      ∀ c₁ c₂ : (container i o s), c₁ = c₂ → process c₁ b = process c₂ b
 
-    theorem deterministic (n : network) : determinism n :=
-      assume (e₁ e₂ : env) (h : e₁ = e₂),
-      show process e₁ n = process e₂ n, from congr (congr_arg process h) (refl n)
+    theorem deterministic (b : body i o s) : determinism b :=
+      assume e₁ e₂ : container i o s,
+      assume h : e₁ = e₂,
+      show process e₁ b = process e₂ b,
+      from congr (congr_arg process h) (refl b)
 
-  end network
+  end body
 
-  -- SEQUENCE NETWORK
+  -- BODY SEQUENCE
 
-  namespace network'
+  namespace body'
     
-    -- Given a list of port assignments, an initial state and a network, `process'` ouputs the environment after the networked has
+    -- Given a list of port assignments, an initial state and a body, `process` outputs the environment after the body has
     -- processed the list of inputs. The `state` output of one reaction is fed as input to the next.
-    def process : (list ports) → state → network → (list env)
+    def process {i o s : ℕ} : list (inputs i × outputs o) → (state s) → (body i o s) → list (container i o s)
       | [] _ _ := []
-      | (list.cons p t) s n := let e' := (network.process ⟨p, s⟩ n) in list.cons e' (process t e'.1 n) 
+      | (list.cons io_h io_t) s b := let c' := body.process ⟨io_h.1, io_h.2, s⟩ b in list.cons c' (process io_t c'.2.2 b) 
 
-    def determinism (n : network) : Prop := 
-      ∀ (p₁ p₂ : list ports) (s₁ s₂ : state), (p₁ = p₂ ∧ s₁ = s₂) → (process p₁ s₁ n) = (process p₂ s₂ n)
+    def determinism {i o s : ℕ} (b : body i o s) : Prop := 
+      ∀ (io₁ io₂ : list (inputs i × outputs o)) (s₁ s₂ : state s), 
+      (io₁ = io₂ ∧ s₁ = s₂) → (process io₁ s₁ b) = (process io₂ s₂ b)
 
-    theorem deterministic (n : network) : determinism n :=
-      assume (p₁ p₂ : list ports) (s₁ s₂ : state) (h : p₁ = p₂ ∧ s₁ = s₂),
-      show process p₁ s₁ n = process p₂ s₂ n, from congr (congr (congr_arg process h.left) h.right) (refl n)
+    theorem deterministic (b : body i o s) : determinism b :=
+      assume io₁ io₂ : list (inputs i × outputs o),
+      assume s₁ s₂ : state s,
+      assume h : io₁ = io₂ ∧ s₁ = s₂,
+      show process io₁ s₁ b = process io₂ s₂ b, 
+      from congr (congr (congr_arg process h.left) h.right) (refl b)
 
-  end network'
+  end body'
 
-  
+  structure reactor :=
+    (d : identifier)
+    (c : container i o s)
+    (b : body i o s)
 
-end determinism
+end hidden
